---
title: "Tarea 5. Pregunta 9.2."
---

Pruebe si $X, Y$ v.a., $a\in\mathbb{R}$ entonces:

9.2.1 $(aX)^{+} + (aY)^{-} \leq |a|(X^{+} + Y^{-})$.

Demostración: 

Sabemos que

\begin{align*}
(aX)^{+} &:= \max\{aX,0\} \\\\
&= \frac{|aX - 0| + aX + 0}{2}\\\\
&= \frac{|a||X| + aX}{2}\\\\
&= |a|\frac{|X| + signo(a)X}{2}\\\\
\end{align*}

De manera análoga :

\begin{align*}
(aX)^{-} &:= \max\{-aX,0\} \\\\
&= \frac{|-aX - 0| - aX + 0}{2}\\\\
&= \frac{|a||X| - aX}{2}\\\\
&= |a|\frac{|X| - signo(a)X}{2}\\\\
\end{align*}

Así

\begin{align*}
(aX)^{+} + (aX)^{-} &:= |a|\frac{|X| + signo(a)X}{2} + |a|\frac{|X| - signo(a)X}{2}\\\\
&= |a|(\frac{|X| + signo(a)X}{2} + \frac{|X| - signo(a)X}{2})\\\\
&= |a||X|\\\\
&= |a|[\max\{aX,0\} + \max\{-aX,0\}]\\\\
&= |a|[(X)^{+} + (X)^{-}].
\end{align*}
Por lo tanto
\begin{align*}
 (aX)^{+} + (aX)^{-} = |a|[(X)^{+} + (X)^{-}].
\end{align*}


9.2.2 $(X + Y)^{+} + (X + Y)^{-} \leq X^{+} + X^{-} + Y^{+} + Y^{-}$.
Observemos que:

\[X^{+} = \max\{X,0\} = \frac{|X|+X}{2}\]
\[X^{-} = \max\{-X,0\} = \frac{|X|-X}{2}\]

Análogamente

\[Y^{+} = \frac{|Y|+Y}{2}\]
\[Y^{-} = \frac{|Y|-Y}{2}\]

Así

\[X^{+} + Y^{+} = \frac{|X| + |Y| + (X + Y)}{2}\]
\[X^{-} + Y^{-} = \frac{|X| + |Y| - (X + Y)}{2}\]

Aplicando la desigualdad del triángulo.

\[X^{+} + Y^{+} = \frac{|X| + |Y| + (X + Y)}{2} \geq \frac{|X + Y| + (X + Y)}{2} = \max\{X+Y,0\} = (X + Y)^{+}\]

\[X^{-} + Y^{-} = \frac{|X| + |Y| - (X + Y)}{2} \geq \frac{|X + Y| - (X + Y)}{2} = \max\{-(X+Y),0\} = (X + Y)^{-}\]

Por lo tanto

\[(X + Y)^{+} + (X + Y)^{-} \leq X^{+} + X^{-} + Y^{+} + Y^{-} \]

